\documentclass[12pt]{article}
\usepackage{amssymb}

\begin{document}

Start with the normalized SIR:

$$ i = Bxy; \dot x = -i; \dot y = i-y $$

If $C(t)$ is the expected case reproductive number for the cohort infected at time $t$, then the overall mean is:

$$
	\bar C
	= \frac{\int{dt\, i(t) C(t)}}{\int{dt\, i(t)}}
	= \frac{\int{dt\, i(t) C(t)}}{Z},
$$

where $Z$ is the size of the epidemic.

Individuals in a cohort are effectively assumed to differ only in terms of how long they are infectious. We calculate $C(t)$ as a weighted average over this duration. The probability of having duration $D$ is just $\exp(-\delta)$ in this normalized model, and the reproductive number for this group is given by:
$$C(t, \delta) = B \int^D{d\delta\, x(t+\delta)}, $$

Thus:
$$C(t) = B \int{d\delta\, x(t+\delta) \exp(-\delta)}, $$
or, in terms of time of contact $\tau=t+\delta$:
$$C(t) = B \int_{\tau>t}{d\tau\, x(\tau) \exp(t-\tau)}, $$

We can also solve the $\dot y$ equation, by looking at who was infected at time $\theta$, and how many of them survived:

$$ y(t) = \int_{\theta<t}{d\theta\, i(\theta)\exp(\theta-t)},$$

and then expand:

\begin{eqnarray}
	Z \bar C
	&=& \int{dt\, i(t) C(t)}
	\\ &=& B \int{dt\, i(t) \int_{\tau>t}{d\tau\, x(\tau) \exp(t-\tau)}}
	\\ &=& B \int{d\tau\, x(\tau) \int_{t<\tau}dt\, i(t) \exp(t-\tau)}
	\\ &=& B \int{d\tau\, x(\tau) y(\tau)}
	\\ &=& \int{d\tau\, i(\tau)}
	\\ &=& Z
\end{eqnarray}

Thus, $\bar C = 1$, as expected. Note: we could presumably fiddle with having a finite $y_0$ by playing with integral limits in the array above to get something like $(Z-x_0)/Z$.

Now try to expand the sum of squares. One trick we're using here is that to compute the square of the integral of $f(x)$ over a range, we can just take twice the integral of $f(x)f(y)$ over a triangle where we assume we know $x>y$.

First, we look only at between-cohort variance, so our first step is to expand the sum of squares there.

\begin{eqnarray}
\int{dt\, i(t) C^2(t)}
	\\ = \int{dt\, i(t) \left(
		B \int_{\tau>t}{d\tau\, x(\tau) \exp(t-\tau)}
	\right)^2}
	\\ = B^2 \int{dt\, i(t) \left(
		\int_{\tau>t}{d\tau\, x(\tau) \exp(t-\tau)}
	\right)^2}
	\\ =  2B^2 \int{dt\, i(t) \int_{\tau>t}{d\tau\, \int_{\sigma>\tau}{d\sigma\, x(\tau) x(\sigma) \exp(t-\tau)\exp(t-\sigma)}}}
\end{eqnarray}

Now, we first integrate over $t$ instead:
  $$ 2B^2 \int{dt\, i(t) \int_{\tau>t}{d\tau\, \int_{\sigma>\tau}{d\sigma\, x(\tau) x(\sigma) \exp(t-\tau)\exp(t-\sigma)}}}$$
  $$ = 2B^2 \int{d\tau\, x(\tau) \int_{\sigma > \tau}{d\sigma\, x(\sigma) \exp(\tau-\sigma)\int_{t<\tau}{dt\, i(t) \exp(t-\tau)}}}$$
Recognizing that the last $dt$ integral is $y(\tau)$ we re-write:
 $$ 2B^2 \int{d\tau\, y(\tau)x(\tau) \int_{\sigma>\tau}{d\sigma\, x(\sigma) \exp(\tau-\sigma)}}$$

Distributing $B$ we see that this is twice expr. (2) = $2Z$.


	% \\ &=& 2B \int{dt\, i(t) \int_{\tau>t}{d\tau\, x(\tau) \exp(t-\tau) C(\tau)}}
	% \\ &=& 2B \int{d\tau\, x(\tau) C(\tau) \int_{t<\tau}{dt\, i(t) \exp(t-\tau)}}
	% \\ &=& 2B \int{d\tau\, x(\tau) C(\tau) y(\tau)}
	% \\ &=& 2 \int{d\tau\, C(\tau) i(\tau)}


% Wait! Does this prove the Roswell Conjecture‽ It \emph{seems} too simple (we haven't seen how far the “proof” would go with a different infectiousness kernel), but maybe we accidentally leveraged the distribution-matching property of the exponential (infectious period has same distribution as generation interval) – that actually seems plausible.
%
% PS: This does balance correctly, fwiw: it yields a squared-sum of $2Z/Z = 2$ to go with the mean of 1, so a variance of 1.

*scribbling
We said above that the individual cases per case $C_i(t) = B\int_{0}^{\delta}{d\tau\, x(t + \tau)}$ and its expectation for a cohort infected at time $t$ is $C(t) = B\int_{0}^{\infty}{d\delta\, x(t+\delta) \exp(-\delta)}$. Let's work on the second moment for $C_i(t)$ for a sec and see if we can make things line up.

$$\mathbb{E}[C^2_i(t)] = B^2 \mathbb{E}\left[\left(
  \int_{0}^{\delta}{d\tau\, x(t+\tau)}\right)^2
  \right]$$

$$ = B^2 \mathbb{E}\left[\left(
  \int_{0}^{\delta}{d\tau\,\int_{0}^{\delta}{d\tau'\, x(t+\tau) x(t+\tau')}}\right)
  \right]$$

I think we are allowed to take the expectation over the exponentially distributed durations

$$= B^2 \int_{0}^{\infty}{d\delta\, exp(-\delta)\int_{0}^{\delta}{d\tau\,\int_{0}^{\delta}{d\tau'\, x(t+\tau) x(t+\tau')}}}$$

Do another triangle trick

$$= 2B^2 \int_{0}^{\infty}{d\delta\, exp(-\delta)\int_{0}^{\delta}{d\tau\,\int_{0}^{\tau}{d\tau'\, x(t+\tau) x(t+\tau')}}}$$

Out of tricks...


\end{document}
